theories/proofmode/solve_pure.v
@@ -37,7 +37,7 @@ Qed.
 
 #[export] Hint Mode isCorrectPC + : solve_pure.
 
-#[export] Hint Resolve isCorrectPC_ExecPCPerm_InBounds : solve_pure.
+(* #[export] Hint Resolve isCorrectPC_ExecPCPerm_InBounds : solve_pure. *)
 
 (* Proxy lemma for DecodeInstr *)
 
@@ -51,21 +51,21 @@ Qed.
 
 (* ExecPCPerm, PermFlowsTo *)
 
-#[export] Hint Mode ExecPCPerm + : solve_pure.
+(* #[export] Hint Mode ExecPCPerm + : solve_pure. *)
 #[export] Hint Mode PermFlowsTo - + : solve_pure.
 
-Lemma ExecPCPerm_InCtx p :
-  InCtx (ExecPCPerm p) → ExecPCPerm p.
-Proof. auto. Qed.
-#[export] Hint Resolve ExecPCPerm_InCtx : solve_pure.
+(* Lemma ExecPCPerm_InCtx p : *)
+(*   InCtx (ExecPCPerm p) → ExecPCPerm p. *)
+(* Proof. auto. Qed. *)
+(* #[export] Hint Resolve ExecPCPerm_InCtx : solve_pure. *)
 
-#[export] Hint Resolve ExecPCPerm_RX : solve_pure.
-#[export] Hint Resolve ExecPCPerm_RWX : solve_pure.
-#[export] Hint Resolve ExecPCPerm_not_E : solve_pure.
-#[export] Hint Resolve ExecPCPerm_flows_to : solve_pure.
-(* TODO: add a test checking the use of ExecPCPerm_flows_to (if it is still
-   needed) *)
-#[export] Hint Resolve ExecPCPerm_readAllowed : solve_pure.
+(* #[export] Hint Resolve ExecPCPerm_RX : solve_pure. *)
+(* #[export] Hint Resolve ExecPCPerm_RWX : solve_pure. *)
+(* #[export] Hint Resolve ExecPCPerm_not_E : solve_pure. *)
+(* #[export] Hint Resolve ExecPCPerm_flows_to : solve_pure. *)
+(* (* TODO: add a test checking the use of ExecPCPerm_flows_to (if it is still *)
+(*    needed) *) *)
+(* #[export] Hint Resolve ExecPCPerm_readAllowed : solve_pure. *)
 (* Will only work if arguments are concrete terms *)
 #[export] Hint Extern 1 (readAllowed _ = true) => reflexivity : solve_pure.
 #[export] Hint Extern 1 (writeAllowed _ = true) => reflexivity : solve_pure.
@@ -116,29 +116,29 @@ Goal forall (r_t1 PC: RegName) `{MachineParameters}, exists r1 r2,
   r1 = r_t1 ∧ r2 = inr PC.
 Proof. do 2 eexists. repeat apply conj. solve_pure. all: reflexivity. Qed.
 
-Goal forall p g b e a,
-  ExecPCPerm p →
-  SubBounds b e a (a ^+ 5)%a →
-  ContiguousRegion a 5 →
-  isCorrectPC (WCap p g b e a).
-Proof. intros. solve_pure. Qed.
+(* Goal forall p g b e a, *)
+(*   ExecPCPerm p → *)
+(*   SubBounds b e a (a ^+ 5)%a → *)
+(*   ContiguousRegion a 5 → *)
+(*   isCorrectPC (WCap p g b e a). *)
+(* Proof. intros. solve_pure. Qed. *)
 
-Goal forall (r_t1 r_t2: RegName), exists r1 r2,
-  is_Get (GetB r_t2 r_t1) r1 r2 ∧
-  r1 = r_t2 ∧ r2 = r_t1.
-Proof. do 2 eexists. repeat apply conj. solve_pure. all: reflexivity. Qed.
+(* Goal forall (r_t1 r_t2: RegName), exists r1 r2, *)
+(*   is_Get (GetB r_t2 r_t1) r1 r2 ∧ *)
+(*   r1 = r_t2 ∧ r2 = r_t1. *)
+(* Proof. do 2 eexists. repeat apply conj. solve_pure. all: reflexivity. Qed. *)
 
-Goal forall p g b e a,
-  ExecPCPerm p →
-  SubBounds b e a (a ^+ 5)%a →
-  ContiguousRegion a 5 →
-  isCorrectPC (WCap p g b e (a ^+ 1)%a).
-Proof. intros. solve_pure. Qed.
+(* Goal forall p g b e a, *)
+(*   ExecPCPerm p → *)
+(*   SubBounds b e a (a ^+ 5)%a → *)
+(*   ContiguousRegion a 5 → *)
+(*   isCorrectPC (WCap p g b e (a ^+ 1)%a). *)
+(* Proof. intros. solve_pure. Qed. *)
 
 Goal forall (r_t1 r_t2 r_t3: RegName), exists r1 r2 r3,
   is_AddSubLt (Sub r_t2 r_t2 r_t3) r1 (inr r2) (inr r3) ∧
   r1 = r_t2 ∧ r2 = r_t2 ∧ r3 = r_t3.
 Proof. do 3 eexists. repeat apply conj. solve_pure. all: reflexivity. Qed.
 
-Goal E ≠ RO. solve_pure. Qed.
+(* Goal E ≠ RO. solve_pure. Qed. *)
 Goal forall (P: Prop), P → P. intros. solve_pure. Qed.
